Resource footprints can now depend on the heap!

pulse/ulib/LowStar.RST.Pointer.Views.fst
@@ -24,7 +24,7 @@ noeq type vptr (a: Type) = {
 abstract
 let ptr_view (#a:Type) (ptr:pointer a) : view (vptr a) =
   reveal_view ();
-  let fp = Ghost.hide (A.loc_array ptr) in
+  let fp (h: HS.mem) = A.loc_array ptr in
   let inv (h: HS.mem): prop = A.live h ptr /\ A.vlength ptr = 1 in
   let sel h = {x = Seq.index (A.as_seq h ptr) 0; p = Ghost.hide (A.get_perm h ptr 0)} in
   {
@@ -37,8 +37,8 @@ let ptr_resource (#a:Type) (ptr:pointer a) =
   as_resource (ptr_view ptr)
 
 let reveal_ptr ()
-  : Lemma ((forall a (ptr:pointer a) .{:pattern as_loc (fp (ptr_resource ptr))}
-             as_loc (fp (ptr_resource ptr)) == A.loc_array ptr) /\
+  : Lemma ((forall a (ptr:pointer a) h .{:pattern as_loc (fp (ptr_resource ptr)) h}
+             as_loc (fp (ptr_resource ptr)) h == A.loc_array ptr) /\
            (forall a (ptr:pointer a) h .{:pattern inv (ptr_resource ptr) h}
              inv (ptr_resource ptr) h <==> A.live h ptr /\ A.vlength ptr = 1) /\
            (forall a (ptr:pointer a) h .{:pattern sel (ptr_view ptr) h}
